more cleanup

src/Init/Data/List/Sort.lean
@@ -24,9 +24,24 @@ theorem splitAt_eq (n : Nat) (l : List α) : splitAt n l = (l.take n, l.drop n) 
   rw [splitAt, splitAt_go, reverse_nil, nil_append]
 
 /--
+`O(min |l| |r|)`. Merge two lists using `le` as a switch.
+
+This version is not tail-recursive,
+but it is replaced at runtime by `mergeTR` using a `@[csimp]` lemma.
+-/
+def merge (le : α → α → Bool) : List α → List α → List α
+  | [], ys => ys
+  | xs, [] => xs
+  | x :: xs, y :: ys =>
+    if le x y then
+      x :: merge le xs (y :: ys)
+    else
+      y :: merge le (x :: xs) ys
+
+/--
 `O(|l| + |r|)`. Merge two lists using `le` as a switch.
 -/
-def merge (le : α → α → Bool) (l₁ l₂ : List α) : List α :=
+def mergeTR (le : α → α → Bool) (l₁ l₂ : List α) : List α :=
   go l₁ l₂ []
 where go : List α → List α → List α → List α
   | [], l₂, acc => reverseAux acc l₂
@@ -45,22 +60,37 @@ def splitInTwo (l : { l : List α // l.length = n }) :
   let r := splitAt ((n+1)/2) l.1
   (⟨r.1, by simp [r, splitAt_eq, l.2]; omega⟩, ⟨r.2, by simp [r, splitAt_eq, l.2]; omega⟩)
 
-def mergeSort (le : α → α → Bool) (l : List α) : List α :=
+/--
+Simplified implementation of stable merge sort.
+
+This version uses the non tail-recursive `merge` function,
+and so is not suitable for large lists, but is straightforward to reason about.
+It is replaced at runtime by `mergeSortTR` using a `@[csimp]` lemma.
+-/
+def mergeSort (le : α → α → Bool) : List α → List α
+  | [] => []
+  | [a] => [a]
+  | a :: b :: xs =>
+    let lr := splitInTwo ⟨a :: b :: xs, rfl⟩
+    have := by simpa using lr.2.2
+    have := by simpa using lr.1.2
+    merge le (mergeSort le lr.1) (mergeSort le lr.2)
+termination_by l => l.length
+
+def mergeSortTR (le : α → α → Bool) (l : List α) : List α :=
   run ⟨l, rfl⟩
 where run : {n : Nat} → { l : List α // l.length = n } → List α
   | 0, ⟨[], _⟩ => []
   | 1, ⟨[a], _⟩ => [a]
   | n+2, xs =>
     let (l, r) := splitInTwo xs
-    merge le (run l) (run r)
+    mergeTR le (run l) (run r)
 
-#eval mergeSort (· ≤ ·) [3, 1, 4, 1, 5, 9, 2, 6, 5, 3, 5]
+#eval mergeSortTR (· ≤ ·) [3, 1, 4, 1, 5, 9, 2, 6, 5, 3, 5]
 
-#eval mergeSort (fun x y => x/10 ≤ y/10) [3, 100 + 1, 4, 100 + 1, 5, 100 + 9, 2, 10 + 6, 5, 10 + 3, 5]
+#eval mergeSortTR (fun x y => x/10 ≤ y/10) [3, 100 + 1, 4, 100 + 1, 5, 100 + 9, 2, 10 + 6, 5, 10 + 3, 5]
 
 abbrev Sorted (r : α → α → Bool) (xs : List α) : Prop := xs.Pairwise (fun x y => r x y)
-
-namespace mergeSort
 
 @[simp] theorem splitInTwo_fst (l : { l : List α // l.length = n }) : (splitInTwo l).1 = ⟨l.1.take ((n+1)/2), by simp [splitInTwo, splitAt_eq, l.2]; omega⟩ := by
   simp [splitInTwo, splitAt_eq]
@@ -73,84 +103,67 @@ theorem splitInTwo_fst_append_splitInTwo_snd (l : { l : List α // l.length = n 
 
 variable {le : α → α → Bool}
 
-def naiveMerge (lt : α → α → Bool) : List α → List α → List α
-  | [], ys => ys
-  | xs, [] => xs
-  | x :: xs, y :: ys =>
-    if lt x y then
-      x :: naiveMerge lt xs (y :: ys)
-    else
-      y :: naiveMerge lt (x :: xs) ys
-
-@[simp] theorem naiveMerge_nil_right (xs : List α) : naiveMerge le xs [] = xs := by
+@[simp] theorem merge_nil_right (xs : List α) : merge le xs [] = xs := by
   induction xs with
-  | nil => simp [naiveMerge]
-  | cons x xs ih => simp [naiveMerge, ih]
+  | nil => simp [merge]
+  | cons x xs ih => simp [merge, ih]
 
-theorem merge_go_eq_naiveMerge : merge.go le l₁ l₂ acc = acc.reverse ++ naiveMerge le l₁ l₂ := by
+theorem mergeTR_go_eq : mergeTR.go le l₁ l₂ acc = acc.reverse ++ merge le l₁ l₂ := by
   induction l₁ generalizing l₂ acc with
-  | nil => simp [merge.go, naiveMerge, reverseAux_eq]
+  | nil => simp [mergeTR.go, merge, reverseAux_eq]
   | cons x l₁ ih₁ =>
     induction l₂ generalizing acc with
-    | nil => simp [merge.go, naiveMerge, reverseAux_eq]
+    | nil => simp [mergeTR.go, merge, reverseAux_eq]
     | cons y l₂ ih₂ =>
-      simp [merge.go, naiveMerge]
+      simp [mergeTR.go, merge]
       split <;> simp [ih₁, ih₂]
 
-theorem merge_eq_naiveMerge : merge le l₁ l₂ = naiveMerge le l₁ l₂ := by
-  simp [merge, merge_go_eq_naiveMerge]
+@[csimp] theorem merge_eq_mergeTR : @merge = @mergeTR := by
+  funext
+  simp [mergeTR, mergeTR_go_eq]
 
-def naiveMergeSort (le : α → α → Bool) : List α → List α
-  | [] => []
-  | [a] => [a]
-  | a :: b :: xs =>
-    let lr := splitInTwo ⟨a :: b :: xs, rfl⟩
-    have := by simpa using lr.2.2
-    have := by simpa using lr.1.2
-    naiveMerge le (naiveMergeSort le lr.1) (naiveMergeSort le lr.2)
-termination_by l => l.length
-
-theorem mergeSort_run_eq_naiveMergeSort : {n : Nat} → (l : { l : List α // l.length = n }) → mergeSort.run le l = naiveMergeSort le l.1
+theorem mergeSortTR_run_eq_mergeSort : {n : Nat} → (l : { l : List α // l.length = n }) → mergeSortTR.run le l = mergeSort le l.1
   | 0, ⟨[], _⟩
-  | 1, ⟨[a], _⟩ => by simp [run, naiveMergeSort]
+  | 1, ⟨[a], _⟩ => by simp [mergeSortTR.run, mergeSort]
   | n+2, ⟨a :: b :: l, h⟩ => by
     cases h
-    simp [run, naiveMergeSort]
-    rw [merge_eq_naiveMerge]
-    rw [mergeSort_run_eq_naiveMergeSort, mergeSort_run_eq_naiveMergeSort]
+    simp [mergeSortTR.run, mergeSort]
+    rw [merge_eq_mergeTR]
+    rw [mergeSortTR_run_eq_mergeSort, mergeSortTR_run_eq_mergeSort]
 
-theorem mergeSort_eq_naiveMergeSort : mergeSort le l = naiveMergeSort le l := by
-  rw [mergeSort, mergeSort_run_eq_naiveMergeSort]
+@[csimp] theorem mergeSort_eq_mergeSortTR : @mergeSort = @mergeSortTR := by
+  funext
+  rw [mergeSortTR, mergeSortTR_run_eq_mergeSort]
 
-theorem mem_naiveMerge {a : α} {xs ys : List α} : a ∈ naiveMerge le xs ys ↔ a ∈ xs ∨ a ∈ ys := by
+theorem mem_merge {a : α} {xs ys : List α} : a ∈ merge le xs ys ↔ a ∈ xs ∨ a ∈ ys := by
   induction xs generalizing ys with
-  | nil => simp [naiveMerge]
+  | nil => simp [merge]
   | cons x xs ih =>
     induction ys with
-    | nil => simp [naiveMerge]
+    | nil => simp [merge]
     | cons y ys ih =>
-      simp only [naiveMerge]
+      simp only [merge]
       split <;> rename_i h
       · simp_all [or_assoc]
       · simp only [mem_cons, or_assoc, Bool.not_eq_true, ih, ← or_assoc]
         apply or_congr_left
         simp only [or_comm (a := a = y), or_assoc]
 
-theorem naiveMerge_sorted
+theorem merge_sorted
     (trans : ∀ {a b c : α}, le a b → le b c → le a c)
     (total : ∀ {a b : α}, !le a b → le b a)
-    (l₁ l₂ : List α) (h₁ : l₁.Sorted le) (h₂ : l₂.Sorted le) : (naiveMerge le l₁ l₂).Sorted le := by
+    (l₁ l₂ : List α) (h₁ : l₁.Sorted le) (h₂ : l₂.Sorted le) : (merge le l₁ l₂).Sorted le := by
   induction l₁ generalizing l₂ with
-  | nil => simpa only [naiveMerge]
+  | nil => simpa only [merge]
   | cons x l₁ ih₁ =>
     induction l₂ with
-    | nil => simpa only [naiveMerge]
+    | nil => simpa only [merge]
     | cons y l₂ ih₂ =>
-      simp only [naiveMerge]
+      simp only [merge]
       split <;> rename_i h
       · apply Pairwise.cons
         · intro z m
-          rw [mem_naiveMerge, mem_cons] at m
+          rw [mem_merge, mem_cons] at m
           rcases m with (m|rfl|m)
           · exact rel_of_pairwise_cons h₁ m
           · exact h
@@ -158,27 +171,12 @@ theorem naiveMerge_sorted
         · exact ih₁ _ h₁.tail h₂
       · apply Pairwise.cons
         · intro z m
-          rw [mem_naiveMerge, mem_cons] at m
+          rw [mem_merge, mem_cons] at m
           rcases m with (⟨rfl|m⟩|m)
           · exact total (by simpa using h)
           · exact trans (total (by simpa using h)) (rel_of_pairwise_cons h₁ m)
           · exact rel_of_pairwise_cons h₂ m
         · exact ih₂ h₂.tail
-
-theorem naiveMergeSort_sorted
-    (trans : ∀ {a b c : α}, le a b → le b c → le a c)
-    (total : ∀ {a b : α}, !le a b → le b a) :
-    (l : List α) → (naiveMergeSort le l).Sorted le
-  | [] => by simp [naiveMergeSort]
-  | [a] => by simp [naiveMergeSort]
-  | a :: b :: xs => by
-    have : (splitInTwo ⟨a :: b :: xs, rfl⟩).1.1.length < xs.length + 1 + 1 := by simp [splitInTwo_fst]; omega
-    have : (splitInTwo ⟨a :: b :: xs, rfl⟩).2.1.length < xs.length + 1 + 1 := by simp [splitInTwo_snd]; omega
-    rw [naiveMergeSort]
-    apply naiveMerge_sorted @trans @total
-    apply naiveMergeSort_sorted trans total
-    apply naiveMergeSort_sorted trans total
-termination_by l => l.length
 
 theorem splitInTwo_fst_sorted (l : { l : List α // l.length = n }) (h : Sorted le l) : Sorted le (splitInTwo l).1 := by
   rw [splitInTwo_fst]
@@ -194,29 +192,16 @@ theorem splitInTwo_fst_le_splitInTwo_snd {l : { l : List α // l.length = n }} (
   intro a b ma mb
   exact h.rel_of_mem_take_of_mem_drop ma mb
 
-theorem naiveMerge_of_le : ∀ {xs ys : List α} (_ : ∀ a b, a ∈ xs → b ∈ ys → le a b),
-    naiveMerge le xs ys = xs ++ ys
+theorem merge_of_le : ∀ {xs ys : List α} (_ : ∀ a b, a ∈ xs → b ∈ ys → le a b),
+    merge le xs ys = xs ++ ys
   | [], ys, _
-  | xs, [], _ => by simp [naiveMerge]
+  | xs, [], _ => by simp [merge]
   | x :: xs, y :: ys, h => by
-    simp only [naiveMerge, cons_append]
-    rw [if_pos, naiveMerge_of_le]
+    simp only [merge, cons_append]
+    rw [if_pos, merge_of_le]
     · intro a b ma mb
       exact h a b (mem_cons_of_mem _ ma) mb
     · exact h x y (mem_cons_self _ _) (mem_cons_self _ _)
-
-theorem naiveMergeSort_of_sorted : ∀ {l : List α} (_ : Sorted le l), naiveMergeSort le l = l
-  | [], _ => by simp [naiveMergeSort]
-  | [a], _ => by simp [naiveMergeSort]
-  | a :: b :: xs, h => by
-    have : (splitInTwo ⟨a :: b :: xs, rfl⟩).1.1.length < xs.length + 1 + 1 := by simp [splitInTwo_fst]; omega
-    have : (splitInTwo ⟨a :: b :: xs, rfl⟩).2.1.length < xs.length + 1 + 1 := by simp [splitInTwo_snd]; omega
-    rw [naiveMergeSort]
-    rw [naiveMergeSort_of_sorted (splitInTwo_fst_sorted ⟨a :: b :: xs, rfl⟩ h)]
-    rw [naiveMergeSort_of_sorted (splitInTwo_snd_sorted ⟨a :: b :: xs, rfl⟩ h)]
-    rw [naiveMerge_of_le (splitInTwo_fst_le_splitInTwo_snd h)]
-    rw [splitInTwo_fst_append_splitInTwo_snd]
-termination_by l => l.length
 
 def stable_le (le : α → α → Bool) (a b : Nat × α) : Bool :=
   if le a.2 b.2 then if le b.2 a.2 then a.1 ≤ b.1 else true else false
@@ -253,59 +238,62 @@ theorem splitInTwo_cons_cons_enumFrom_snd (i : Nat) (l : List α) :
       congr
       ext <;> simp; omega
 
-theorem naiveMerge_stable : ∀ (xs ys) (_ : ∀ x y, x ∈ xs → y ∈ ys → x.1 ≤ y.1),
-    (naiveMerge (stable_le le) xs ys).map (·.2) = naiveMerge le (xs.map (·.2)) (ys.map (·.2))
-  | [], ys, _ => by simp [naiveMerge]
-  | xs, [], _ => by simp [naiveMerge]
+theorem merge_stable : ∀ (xs ys) (_ : ∀ x y, x ∈ xs → y ∈ ys → x.1 ≤ y.1),
+    (merge (stable_le le) xs ys).map (·.2) = merge le (xs.map (·.2)) (ys.map (·.2))
+  | [], ys, _ => by simp [merge]
+  | xs, [], _ => by simp [merge]
   | (i, x) :: xs, (j, y) :: ys, h => by
-    simp only [naiveMerge, stable_le, map_cons]
+    simp only [merge, stable_le, map_cons]
     split <;> rename_i w
     · rw [if_pos (by simp [h _ _ (mem_cons_self ..) (mem_cons_self ..)])]
       simp only [map_cons, cons.injEq, true_and]
-      rw [naiveMerge_stable, map_cons]
+      rw [merge_stable, map_cons]
       exact fun x' y' mx my => h x' y' (mem_cons_of_mem (i, x) mx) my
     · simp only [↓reduceIte, map_cons, cons.injEq, true_and]
-      rw [naiveMerge_stable, map_cons]
+      rw [merge_stable, map_cons]
       exact fun x' y' mx my => h x' y' mx (mem_cons_of_mem (j, y) my)
 
 -- TODO: replace this with a proof via `Perm`
-@[simp] theorem mem_naiveMergeSort {a : α} {l : List α} : a ∈ naiveMergeSort le l ↔ a ∈ l := by
+@[simp] theorem mem_mergeSort {a : α} {l : List α} : a ∈ mergeSort le l ↔ a ∈ l := by
   sorry
 
-theorem naiveMergeSort_stable : ∀ {i : Nat} {l : List α},
-    (naiveMergeSort (stable_le le) (l.enumFrom i)).map (·.2) = naiveMergeSort le l
-  | _, []
-  | _, [a] => by simp [naiveMergeSort]
-  | _, a :: b :: xs => by
-    have : (splitInTwo ⟨a :: b :: xs, rfl⟩).1.1.length < xs.length + 1 + 1 := by simp [splitInTwo_fst]; omega
-    have : (splitInTwo ⟨a :: b :: xs, rfl⟩).2.1.length < xs.length + 1 + 1 := by simp [splitInTwo_snd]; omega
-    simp only [naiveMergeSort, enumFrom]
-    rw [splitInTwo_cons_cons_enumFrom_fst]
-    rw [splitInTwo_cons_cons_enumFrom_snd]
-    rw [naiveMerge_stable]
-    · rw [naiveMergeSort_stable, naiveMergeSort_stable]
-    · simp only [mem_naiveMergeSort, Prod.forall]
-      intros j x k y mx my
-      have := mem_enumFrom mx
-      have := mem_enumFrom my
-      simp_all
-      omega
-termination_by _ l => l.length
+/--
+The result of `mergeSort` is sorted,
+as long as the comparison function is transitive (`le a b → le b c → le a c`)
+and total in the sense that `le a b ∨ le b a`.
 
-end mergeSort
-
-open mergeSort
-
+The comparison function need not be irreflexive, i.e. `le a b` and `le b a` is allowed even when `a ≠ b`.
+-/
 theorem mergeSort_sorted
     (trans : ∀ {a b c : α}, le a b → le b c → le a c)
-    (total : ∀ {a b : α}, !le a b → le b a)
-    (l : List α) : (mergeSort le l).Sorted le := by
-  rw [mergeSort_eq_naiveMergeSort]
-  apply naiveMergeSort_sorted @trans @total
+    (total : ∀ {a b : α}, !le a b → le b a) :
+    (l : List α) → (mergeSort le l).Sorted le
+  | [] => by simp [mergeSort]
+  | [a] => by simp [mergeSort]
+  | a :: b :: xs => by
+    have : (splitInTwo ⟨a :: b :: xs, rfl⟩).1.1.length < xs.length + 1 + 1 := by simp [splitInTwo_fst]; omega
+    have : (splitInTwo ⟨a :: b :: xs, rfl⟩).2.1.length < xs.length + 1 + 1 := by simp [splitInTwo_snd]; omega
+    rw [mergeSort]
+    apply merge_sorted @trans @total
+    apply mergeSort_sorted trans total
+    apply mergeSort_sorted trans total
+termination_by l => l.length
 
-theorem mergeSort_of_sorted (h : Sorted le l) : mergeSort le l = l := by
-  rw [mergeSort_eq_naiveMergeSort]
-  apply naiveMergeSort_of_sorted h
+/--
+If the input list is already sorted, then `mergeSort` does not change the list.
+-/
+theorem mergeSort_of_sorted : ∀ {l : List α} (_ : Sorted le l), mergeSort le l = l
+  | [], _ => by simp [mergeSort]
+  | [a], _ => by simp [mergeSort]
+  | a :: b :: xs, h => by
+    have : (splitInTwo ⟨a :: b :: xs, rfl⟩).1.1.length < xs.length + 1 + 1 := by simp [splitInTwo_fst]; omega
+    have : (splitInTwo ⟨a :: b :: xs, rfl⟩).2.1.length < xs.length + 1 + 1 := by simp [splitInTwo_snd]; omega
+    rw [mergeSort]
+    rw [mergeSort_of_sorted (splitInTwo_fst_sorted ⟨a :: b :: xs, rfl⟩ h)]
+    rw [mergeSort_of_sorted (splitInTwo_snd_sorted ⟨a :: b :: xs, rfl⟩ h)]
+    rw [merge_of_le (splitInTwo_fst_le_splitInTwo_snd h)]
+    rw [splitInTwo_fst_append_splitInTwo_snd]
+termination_by l => l.length
 
 /--
 This merge sort algorithm is stable,
@@ -314,17 +302,51 @@ has no effect on the output.
 
 That is, elements which are equal with respect to the ordering function will remain
 in the same order in the output list as they were in the input list.
+
+See also:
+* `mergeSort_stable_pair`: if `[a, b] <+ l` and `le a b`, then `[a, b] <+ mergeSort le l`)
+* `mergeSort_stable_sublist`: if `c <+ l` and `c.Pairwise le`, then `c <+ mergeSort le l`.
 -/
-theorem mergeSort_stable {l : List α} :
-    let stable_le := fun a b => if le a.2 b.2 then if le b.2 a.2 then a.1 ≤ b.1 else true else false
-    (mergeSort stable_le l.enum).map (·.2) = mergeSort le l := by
-  dsimp [stable_le]
-  rw [mergeSort_eq_naiveMergeSort, mergeSort_eq_naiveMergeSort]
-  erw [naiveMergeSort_stable] -- `erw` here to make the `stable_le` definitions match
+theorem mergeSort_stable : ∀ {i : Nat} {l : List α},
+    (mergeSort (stable_le le) (l.enumFrom i)).map (·.2) = mergeSort le l
+  | _, []
+  | _, [a] => by simp [mergeSort]
+  | _, a :: b :: xs => by
+    have : (splitInTwo ⟨a :: b :: xs, rfl⟩).1.1.length < xs.length + 1 + 1 := by simp [splitInTwo_fst]; omega
+    have : (splitInTwo ⟨a :: b :: xs, rfl⟩).2.1.length < xs.length + 1 + 1 := by simp [splitInTwo_snd]; omega
+    simp only [mergeSort, enumFrom]
+    rw [splitInTwo_cons_cons_enumFrom_fst]
+    rw [splitInTwo_cons_cons_enumFrom_snd]
+    rw [merge_stable]
+    · rw [mergeSort_stable, mergeSort_stable]
+    · simp only [mem_mergeSort, Prod.forall]
+      intros j x k y mx my
+      have := mem_enumFrom mx
+      have := mem_enumFrom my
+      simp_all
+      omega
+termination_by _ l => l.length
+
+/--
+Another statement of stability of merge sort.
+If a pair `[a, b]` is a sublist of `l` and `le a b`,
+then `[a, b]` is still a sublist of `mergeSort le l`.
+-/
+theorem mergeSort_stable_pair (h : [a, b] <+ l) (hab : le a b) : [a, b] <+ mergeSort le l := by
+  sorry
+
+/--
+Another statement of stability of merge sort.
+If `c` is a sublist of `l` and `c` is pairwise `le`,
+then `c` is still a sublist of `mergeSort le l`.
+-/
+theorem mergeSort_stable_antichain {c : List α} (hc : c.Pairwise (fun a b => le a b)) (h : c <+ l) :
+    c <+ mergeSort le l := by
+  sorry
 
 end List
 
 open List
 
--- #time
--- #eval (mergeSort (· ≤ ·) (iota (10^7))).length
+#time
+#eval (mergeSort (· ≤ ·) (iota (10^6))).length
